some work

src/tactic/back/interactive.lean
@@ -6,10 +6,14 @@ namespace interactive
 open back
 open interactive interactive.types lean.parser
 
-meta def back (lemmas : parse (optional $ list_of ident)) : tactic unit :=
-do lemmas ← lemmas.to_list.join.mmap (λ n, tactic.resolve_name n >>= tactic.i_to_expr_for_apply),
-   let cfg : config := {passed_lemmas := lemmas},
-   search cfg
+meta def back (should_trace : parse $ optional (tk "?"))
+  (lemmas : parse $ optional $ list_of ident) : tactic unit :=
+do prev ← save_tracing should_trace.is_some,
+
+   lemmas ← lemmas.to_list.join.mmap (λ n, tactic.resolve_name n >>= tactic.i_to_expr_for_apply),
+   search { passed_lemmas := lemmas },
+
+   restore_tracing prev
 
 end interactive
 end tactic
