test/back/primes.lean
@@ -1,0 +1,59 @@
+import tactic.back
+import data.nat.prime
+
+open nat
+
+attribute [back] ne_of_gt le_of_lt nat.dvd_add_iff_right prime.pos prime.not_dvd_one
+-- attribute [back!] succ_lt_succ fact_pos min_fac_prime min_fac_dvd
+attribute [back] succ_lt_succ fact_pos min_fac_prime min_fac_dvd
+attribute [back] dvd_fact
+
+theorem infinitude_of_primes : ∀ N, ∃ p ≥ N, prime p :=
+begin
+  intro N,
+  let M := fact N + 1,
+  let p := min_fac M,
+
+  have pp : prime p := min_fac_prime (ne_of_gt (succ_lt_succ (fact_pos N))),
+
+  use p,
+  split,
+  { by_contradiction,
+    simp at a,
+    have h₁ : p ∣ M := min_fac_dvd M,
+    have h₂ : p ∣ fact N := dvd_fact (prime.pos pp) (le_of_lt a),
+    have h : p ∣ 1 := (nat.dvd_add_iff_right h₂).mpr h₁,
+    exact prime.not_dvd_one pp h, },
+  { assumption }
+end
+
+example : ∀ N, ∃ p ≥ N, prime p :=
+begin
+  intro N,
+  let M := fact N + 1,
+  let p := min_fac M,
+
+  have pp : prime p := by back,
+
+  use p,
+  split,
+  { by_contradiction,
+    simp at a,
+    have h₁ : p ∣ M, by back,
+    have h₂ : p ∣ fact N, by back,
+    -- have h : p ∣ 1 := (nat.dvd_add_iff_right h₂).mpr h₁,
+    have h : p ∣ 1, by back, -- This one makes us take a trip to struggletown
+    back },
+  { assumption }
+end
+
+example (N : ℕ) : ∃ p ≥ N, prime p :=
+begin
+  use min_fac (fact N + 1),
+  split,
+  { by_contradiction h, simp at h,
+    -- apply prime.not_dvd_one,
+    -- back
+  },
+  back
+end
